Continue the proof of the Lemma 5.

Coq/src/drf/DRF_RLX.v
@@ -19,6 +19,10 @@ Definition program_execution P S X :=
 Definition RLX_race_free_program P :=
   (forall S X, program_execution P S X -> Race.rc11_consistent_x S X -> Race.RLX_race_free S X).
 
+
+Definition HB_prefix S v1 v2 := dom_rel (S.(hb)^? ⨾ (⦗eq v1⦘ ∪ ⦗eq v2⦘)). 
+
+
 Lemma wf_es P
       (S : ES.t)
       (STEPS : (step Weakestmo)＊ (prog_es_init P) S):
@@ -46,34 +50,93 @@ Proof.
                                        (prog_es_init P)
                                        (fun s => s.(ES.jf) ⊆ s.(hb))).
   intro H. apply H. 1, 3: auto; basic_solver.
-  clear H STEPS S. intros G G' STEPS IH STEP. 
-  assert (WF : ES.Wf G').
-  { eapply wf_es with (P := P). eapply transitive_rt. 2: apply rt_step. all: eauto. } 
+  clear H STEPS S. intros G G' STEPS IH STEP.
+  
+  assert (WF_G : ES.Wf G).
+  { eapply wf_es; eauto. }
+  assert (WF_G' : ES.Wf G').
+  { eapply wf_es. eapply transitive_rt. 2: apply rt_step. all: eauto. } 
   
   inversion_clear STEP as [e H]. destruct H as [e']. desc. 
-  assert (q: G.(hb) ⊆ G'.(hb)). { admit. }
-  inversion_clear TT as [H | [H | [H | H]]].
-  1, 3: inversion_clear H; desc; rewrite JF'; basic_solver. 
-  { inversion_clear H as [w]; desc.
-    assert (hh : (G'.(hb)⁼ w e) \/ (not (G'.(hb)⁼ w e))) by admit. 
-    destruct hh as [[eq_w_e | [ hb_w_e | hb_e_w]] | not_hb_w_e].
-    { admit. }
-    { inversion_clear AJF; desc. rewrite JF'. apply inclusion_union_l.
+  assert (q: G.(hb) ⊆ G'.(hb)).
+  { eapply step_hb_mon; eauto. }
+  inversion_clear TT as [S | [S | [S | S]]].
+  1, 3: inversion_clear S; desc; rewrite JF'; basic_solver. 
+  { 
+    inversion S as [w]; desc.
+    inversion_clear AJF. desf.
+    assert (NCF: ~ (cf G') w e) by auto. 
+    assert (W_w : is_w (lab G') w). 
+    { eapply load_step_W; eauto. intuition. }
+    assert (E_r : is_r (lab G') e) by auto.
+    assert (HB : (G'.(hb)⁼ w e) \/ (not (G'.(hb)⁼ w e))) by apply classic.
+    assert (JF : jf G' w e).
+    { apply JF'. apply inclusion_union_r2. basic_solver. }
+
+    destruct HB as [[EQ_W_E | [ HB_W_E | HB_E_W]] | NOT_HB_W_E].
+    { exfalso. SearchAbout ES.acts_set.
+      eapply BasicStep.basic_step_acts_set_ne; eauto.
+      rewrite <- EQ_W_E. auto. }
+    { rewrite JF'. apply inclusion_union_l.
       { basic_solver. }
       unfold AddJF.jf_delta. basic_solver. }         
-    { exfalso.
-      inversion_clear BSTEP.
-      assert (coh : (irreflexive (G'.(hb) ⨾ (G'.(eco) Weakestmo)^?))).
-      { apply coh. auto. }
-      destruct coh with (x := e).
-      unfold "⨾". exists w. split.
-      { basic_solver. }
-      { apply r_step. unfold eco. apply ct_step.
+    { exfalso. eapply coh; eauto.
+      eexists. split; eauto.
+      apply r_step. unfold eco. apply ct_step.
         repeat apply inclusion_union_r1.
-        unfold ES.rf. unfold "\". split.
-        { unfold "⨾". exists w. split.
-          { apply ES.ew_refl; eauto. inversion AJF. desc. admit. }
-          admit.
+        unfold ES.rf. unfold "\". split; auto.
+        unfold "⨾". exists w. split; auto.
+        apply ES.ew_refl; eauto. 
+        assert (SAME_W : ⦗E G' ∩₁ W G'⦘ ≡ ⦗E G ∩₁ W G⦘).
+        { apply eqv_rel_more. eapply load_step_W; eauto. } 
+        apply SAME_W. desf. }
+    exfalso.
+    set (A := HB_prefix G' e w).
+    assert (PREF_EXEC : program_execution P G' A).
+    { split; unfold A; unfold HB_prefix.
+      all: admit. }
+    assert (PREF_RC11 : Race.rc11_consistent_x G' A).
+    { unfold Race.rc11_consistent_x. admit. }
+    
+    specialize (RACE_FREE G' A PREF_EXEC PREF_RC11).
+    
+    assert (RACE_W : Race.race G' A w).
+    { unfold Race.race. unfold dom_rel. exists e. unfolder. splits.
+      1, 2: unfold A; unfold HB_prefix; basic_solver 10. 
+      apply or_not_and. left. apply or_not_and. left. apply and_not_or. auto. }
+
+    assert (RACE_E : Race.race G' A e).
+    { unfold Race.race. unfold dom_rel. exists w. unfolder. splits.
+      1, 2: unfold A; unfold HB_prefix; basic_solver 10. 
+      apply or_not_and. left. apply or_not_and. left. apply and_not_or. split.
+      { unfolder in NOT_HB_W_E. intuition. }
+      intro. apply ES.cf_sym in H0. auto. }
+    specialize (RACE_FREE w RACE_W) as QW.
+    specialize (RACE_FREE e RACE_E) as QE.
+    destruct QE as [False_W | True_W]; destruct QW as [True_E | False_E].
+    1, 2, 4: try unfolder in False_W; try unfolder in False_E; desf;
+      unfold is_w, is_r in *; basic_solver.
+    apply proj1 in True_E. apply proj1 in True_W.
+    unfold Race.RLX_race_free in RACE_FREE.
+    unfolder in NOT_HB_W_E. apply NOT_HB_W_E. right. left.
+    unfold hb. apply ct_step. apply inclusion_union_r2. unfold sw.
+    unfold "⨾".
+    exists w. split.
+    { unfold release. unfold "⨾".
+      exists w. split.
+      { basic_solver. }
+      exists w. split; auto.
+      unfold rs. unfold "⨾".
+      exists w. split.
+      { unfolder. splits; auto. 
+        eapply BasicStep.basic_step_acts_set_mon; eauto. }
+      exists w. split; auto.
+      exists w. split.
+      { basic_solver. }
+      apply reflexive_rt. }
+    exists e. split; auto.
+    exists e. split; basic_solver. }
+  admit. 
 
 Admitted.
 
@@ -81,7 +144,7 @@ Lemma rf_in_jf (S : ES.t) (X : eventid -> Prop)
       (WF : ES.Wf S)
       (EXEC : Execution.t S X)
       (JF_IN_HB : S.(ES.jf) ⊆ S.(hb)):
-  (⦗X⦘ ⨾ S.(ES.rf) ⨾ ⦗X⦘) ⊆ S.(ES.jf).
+  ⦗X⦘ ⨾ S.(ES.rf) ⨾ ⦗X⦘ ⊆ S.(ES.jf).
 Proof.
   unfolder; intros x y H. 
   destruct H as [x_in_X [rf_x_y y_in_X]].
